Proof homomorphism on set union

VeriSkel/SeqSkel.v
@@ -529,6 +529,437 @@ End VarA_eq.
 Module SE := MSetWeakList.Make VarE_eq.
 Module SA := MSetWeakList.Make VarA_eq.
 
+Module Type DecType <: DecidableType.
+  Parameter t : Type.
+  Definition eq := @eq t.
+  Lemma eq_equiv : Equivalence eq.
+    repeat constructor; unfolds; unfold eq; intros; congruence.
+  Qed.
+  Parameter eq_dec : forall x y : t, {x = y} + {x <> y}.
+End DecType.
+
+Require Import SetoidClass.
+
+Module VarsCondition (D : DecType) (Val : DecType).
+  Instance eq_type_dt : eq_type D.t := {| eq_dec := D.eq_dec |}.
+  Instance eq_type_vt : eq_type Val.t := {| eq_dec := Val.eq_dec |}.
+  
+  Module SE := MSetWeakList.Make D.
+
+  Close Scope exp_scope.
+  Infix "==" := equiv.
+
+  Instance eqset_setoid : Setoid SE.t :=
+    {| equiv := SE.Equal; setoid_equiv := _ |}.
+
+  Lemma eqset_empty s s' : SE.Empty s -> s == s' -> SE.Empty s'.
+  Proof.
+    unfold not, SE.Empty, "=="; firstorder.
+  Qed.
+
+  Lemma choose_remove s x : SE.In x s -> s == SE.add x (SE.remove x s).
+  Proof.
+    revert s x; clear; intros s x; simpl.
+    unfold SE.Equal; intros.
+    rewrite SE.add_spec, SE.remove_spec.
+    lets [? | ?]: (eq_dec a x); split; intros; substs; intuition.
+  Qed.
+
+  Lemma equal_in x s s' : SE.In x s -> s == s' -> SE.In x s'.
+  Proof.
+    unfold SE.Equal, SE.In; intros.
+    apply H0; auto.
+  Qed.
+
+  Lemma cardinal0_empty s : SE.cardinal s = 0 <-> SE.Empty s.
+  Proof.
+    unfold SE.Empty, SE.cardinal; intros; split; intros H.
+    - destruct s as [[|? ?] ?]; simpl in *; try congruence.
+      cbv; inversion 1.
+    - destruct s as [[| ? ? ] ?]; simpl; auto.
+      false; lets: (H e); apply H0; left; auto.
+  Qed.
+
+  Lemma cardinal_add x s : ~SE.In x s -> SE.cardinal (SE.add x s) = S (SE.cardinal s).
+  Proof.
+    destruct s as [s ?]; unfold SE.In, SE.add, SE.cardinal; simpl.
+    remember (SE.Raw.cardinal s) as car_s eqn:Heqc.
+    clear is_ok.
+    revert s Heqc; induction car_s using lt_wf_ind; intros s Heqc Hnin.
+    destruct car_s.
+    - unfold SE.cardinal in *; destruct s as [|? ?]; simpl in *; congruence.
+    - unfold SE.cardinal in *; destruct s as [|? ?]; simpl in *; try congruence.
+      destruct (D.eq_dec x e); simpl in *; substs.
+      + false; unfold SE.Raw.In in Hnin; apply Hnin.
+        constructor; auto.
+      + forwards* :(>>H car_s s).
+        intros Hc; apply Hnin; right; auto.
+  Qed.  
+
+  Lemma remove_nin x s : ~SE.In x (SE.remove x s).
+  Proof.
+    rewrite SE.remove_spec; intros [? ?]; congruence.
+  Qed.
+
+  Lemma eqset_cardinal s s' : s == s' -> SE.cardinal s = SE.cardinal s'.
+  Proof.
+    destruct s as [s oks], s' as [s' oks'].
+    simpl; unfold SE.Equal, SE.In, SE.cardinal.
+    revert s' oks'; induction s; simpl in *; intros s' oks'.
+    - destruct s'; simpl; auto.
+      intros H; lets [? ?]: (H e); unfold SE.Raw.In in *; simpl in *.
+      false; forwards: H1; [left; auto|inversion H2].
+    - intros Heq.
+      inverts oks.
+      assert (SE.Raw.Ok s) by apply H2.
+      cutrewrite (SE.Raw.cardinal s' = S (SE.Raw.cardinal (SE.Raw.remove a s'))).
+      erewrite IHs; eauto using SE.Raw.remove_ok.
+      { intros b; rewrite SE.Raw.remove_spec; eauto.
+        split; intros.
+        + split.
+          rewrite <-Heq; right; auto.
+          intros Hc; substs; unfold SE.Raw.In in *; auto.
+        + destruct H0.
+          rewrite <-Heq in H0; inverts H0; try congruence.
+          unfold SE.Raw.In; auto. }
+      { assert (SE.Raw.In a s').
+        { rewrite <-Heq; left; auto. }
+        revert H0 oks'; clear.
+        induction s'; simpl.
+        - inversion 1.
+        - destruct D.eq_dec as [Heq | Heq]; unfold VarE_eq.eq in Heq; substs; auto.
+          simpl.
+          intros; rewrite <-IHs'; eauto.
+          inversion H0; substs; eauto; congruence.
+          inversion oks'; substs; auto. }
+  Qed.
+
+  Lemma eqset_remove a s s' : s == s' -> SE.remove a s == SE.remove a s'.
+  Proof.
+    simpl; unfold SE.Equal; intros; rewrite !SE.remove_spec.
+    firstorder.
+  Qed.
+
+  Lemma add_eq a s :
+    ~In a s ->
+    SE.Raw.add a s = s ++ a :: nil.
+  Proof.
+    induction s; simpl; eauto.
+    intros Hc.
+    destruct D.eq_dec; simpl.
+    - false; apply Hc; left; auto.
+    - f_equal; rewrite IHs; auto.
+  Qed.
+
+  Lemma set_eq s s' H H' : s = s' -> {| SE.this := s; SE.is_ok := H |} = {| SE.this := s'; SE.is_ok := H' |}.
+  Proof.
+    intros Heq.
+    destruct Heq.
+    assert (H = H') by (apply proof_irrelevance); substs; eauto.
+  Qed.
+
+  Lemma add_spec' a b s :
+    SE.In a (SE.add b s) <-> a = b \/ (a <> b /\ SE.In a s).
+  Proof.
+    splits; [|rewrite SE.add_spec; intros [?|[? ?]]; eauto].
+    destruct s as [s ok]; unfold SE.In, SE.add; simpl.
+    induction s; simpl.
+    - intros H; inverts H as H; eauto.
+      inverts H.
+    - destruct D.eq_dec as [Heq | Hneq]; [substs|].
+      + destruct (eq_dec a a0); eauto.
+      + unfold VarE_eq.eq in Hneq.
+        intros H; inverts H; [right; split; eauto|].
+        * left; eauto.
+        * inverts ok; forwards*: IHs.
+          destruct H as [? | [? ?]]; eauto.
+          right; split; eauto.
+          right; eauto.
+  Qed.
+
+  Lemma add_already a s :
+    SE.In a s -> SE.add a s = s.
+  Proof.
+    destruct s as [s ok]; unfold SE.In, SE.add; simpl.
+    induction s; simpl.
+    - inversion 1.
+    - intros H.
+      apply set_eq.
+      destruct D.eq_dec; eauto.
+      inverts H.
+      unfold VarE_eq.eq in n; congruence.
+      inverts ok.
+      forwards * :(IHs H3).
+      apply (f_equal SE.this) in H; simpl in *; congruence.
+  Qed.
+  
+  Lemma add_inverts a s s' :
+    ~SE.In a s -> ~SE.In a s' ->
+    SE.add a s == SE.add a s' -> s == s'.
+  Proof.
+    unfold "=="; intros ? ? H b.
+    lets ? ?: (H b); rewrite !SE.add_spec in *.
+    split; intros H';
+      [lets [?|?]: (H2 (or_intror H')) | lets [?|?]: (H3 (or_intror H'))]; eauto;
+        [assert (a <> b); [intros Hc; substs; eauto|congruence ]..].
+  Qed.
+  
+  Lemma choose_card s :
+    0 < SE.cardinal s -> exists v, SE.In v s.
+  Proof.
+    destruct s as [[|a s] ok].
+    - unfold SE.cardinal; simpl; omega.
+    - exists a; cbv.
+      left; auto.
+  Qed.
+
+  Lemma remove_card a s :
+    SE.In a s ->
+    SE.cardinal (SE.remove a s) = SE.cardinal s - 1.
+  Proof.
+    intros H; forwards*: (choose_remove s a).
+    lets: (>>eqset_cardinal H0).
+    rewrite cardinal_add in H1; [|apply remove_nin].
+    omega.
+  Qed.
+
+  Lemma union_emp_l s : SE.union SE.empty s == s.
+  Proof.
+    unfold SE.Equal; intros a.
+    rewrite SE.union_spec.
+    lets: (SE.empty_spec); unfold SE.Empty in H.
+    split; [intros [|]|intros]; eauto.
+    intros; false; eapply H; eauto.
+  Qed.
+
+  Lemma union_emp_r s : SE.union s SE.empty == s.
+  Proof.
+    unfold SE.Equal; intros a.
+    rewrite SE.union_spec.
+    lets: (SE.empty_spec); unfold SE.Empty in H.
+    split; [intros [|]|intros]; eauto.
+    intros; false; eapply H; eauto.
+  Qed.
+
+  Lemma cardinal0_empty' s :
+    SE.cardinal s = 0 -> s = SE.empty.
+  Proof.
+    destruct s as [[|a s ] ok]; cbv; try omega.
+    intros; apply set_eq; auto.
+  Qed.
+
+  Lemma diff_emp_r s : SE.diff s SE.empty == s.
+  Proof.
+    unfold "=="; intros a; rewrite SE.diff_spec.
+    lets: SE.empty_spec; unfold SE.Empty in *; firstorder.
+  Qed.
+
+  Instance union_proper_l : Proper (SE.Equal ==> SE.Equal ==> SE.Equal) SE.union.
+  Proof.
+    unfold SE.Equal; intros s1 s2 Heq s3 s4 Heq' a.
+    rewrite !SE.union_spec; firstorder.
+  Qed.
+
+  Instance diff_proper_l : Proper (SE.Equal ==> SE.Equal ==> SE.Equal) SE.diff.
+  Proof.
+    unfold SE.Equal; intros s1 s2 Heq s3 s4 Heq' a.
+    rewrite !SE.diff_spec; firstorder.
+  Qed.
+
+  Instance add_proper_l a : Proper (SE.Equal ==> SE.Equal) (SE.add a).
+  Proof.
+    unfold SE.Equal; intros s1 s2 Heq a'.
+    rewrite !SE.add_spec; firstorder.
+  Qed.
+
+  Variable find : D.t -> option Val.t.
+  Variable den : D.t -> Val.t -> assn.
+
+  Definition assn_of_vs s :=
+    SE.fold (fun x rec =>
+               match find x with
+               | Some vs => den x vs ** rec
+               | None => FalseP
+               end) s emp.
+  
+  Tactic Notation "simpl_avs" "in" hyp(HP) := unfold assn_of_vs, SE.fold in HP; simpl in HP.
+  Tactic Notation "simpl_avs" := unfold assn_of_vs, SE.fold; simpl.
+  Tactic Notation "simpl_avs" "in" "*" := unfold assn_of_vs, SE.fold in *; simpl in *.
+
+  Arguments flip / _ _ _ _ _ _.
+
+  Lemma assn_empty s stk : SE.Empty s -> stk ||= assn_of_vs s <=> emp.
+  Proof.
+    destruct s as [[| ? ?] ?]; rewrite <-SE.is_empty_spec; simpl; 
+      simpl_avs; unfold SE.is_empty; simpl; try congruence.
+    reflexivity.
+  Qed.
+
+  Lemma assn_empty' stk : stk ||= assn_of_vs SE.empty <=> emp.
+  Proof.
+    cbv; eauto.
+  Qed.
+
+  Lemma add_equiv a s stk :
+    ~SE.In a s ->
+    stk ||= assn_of_vs (SE.add a s) <=>
+        match find a with
+        | Some v => den a v ** assn_of_vs s
+        | None => FalseP 
+        end.
+  Proof.
+    unfold assn_of_vs, SE.add, SE.In; rewrite !SE.fold_spec.
+    destruct s as [s oks]; simpl.
+    intros; rewrite add_eq; [|intros Hc; eapply In_InA in Hc; eauto using SE.E.eq_equiv].
+    rewrite fold_left_app; simpl.
+    destruct (find a); [|reflexivity].
+    reflexivity.
+  Qed.
+
+  Lemma fold_left_assns (s : list D.t) (P : assn) (stk : stack):
+    stk ||=
+        fold_left (fun rec x => match find x with
+                                         | Some v => den x v ** rec
+                                         | None => FalseP end) s P <=>
+        P ** fold_left (fun rec x => match find x with
+                                     | Some v => den x v ** rec
+                                     | None => FalseP end) s emp.
+  Proof.
+    revert P; induction s; simpl; intros P.
+    - rewrite emp_unit_r; reflexivity.
+    - rewrite IHs.
+      destruct (find a); simpl.
+      rewrite (IHs (_ ** emp)).
+      repeat rewrite <-sep_assoc, emp_unit_r; split; intros; repeat sep_cancel.
+      rewrite (IHs FalseP).
+      split; intros; destruct H as (? & ? & ? & ? & ?);
+        try lazymatch goal with [H : False|- _] => destruct H end.
+      destruct H0 as (? & ? & ? & ? & ?);
+        try lazymatch goal with [H : False|- _] => destruct H end.
+  Qed.
+
+  Lemma add_equiv'   a s stk :
+    SE.In a s ->
+    stk ||= assn_of_vs s <=>
+            assn_of_vs (SE.add a (SE.remove a s)).
+  Proof.
+    destruct s as [s oks].
+    unfold "==", SE.In, SE.cardinal; simpl.
+    unfold assn_of_vs, SE.fold, SE.Raw.fold at 1; simpl.
+    generalize emp; induction s;  intros P Hin.
+    - inversion Hin.
+    - inverts Hin.
+      + simpl; destruct D.eq_dec as [? | Hneq].
+        2: unfold VarE_eq.eq in Hneq; congruence.
+        rewrite add_eq; [|inverts oks; rewrite InA_alt in *; eauto].
+        unfold SE.Raw.fold; rewrite fold_left_app; simpl.
+        destruct (find a0); simpl.
+        * rewrite fold_left_assns. rewrites (>>fold_left_assns s P).
+          rewrite <-sep_assoc; reflexivity.
+        * rewrite fold_left_assns; split; [|destruct 1].
+          intros (? & ? & ? & ? & ?); eauto.
+      + inverts keep oks.
+        forwards*: (>> (IHs H3)).
+        simpl; rewrite H.
+        assert (a <> a0).
+        { intros Hc; substs; eauto. }
+        destruct D.eq_dec; try congruence.
+        simpl; destruct D.eq_dec; try congruence; simpl.
+        destruct (find a0); [|reflexivity].
+        reflexivity.
+  Qed.
+
+  Lemma eqset_equiv   s s' stk :
+    SE.Equal s s' ->
+    stk ||= assn_of_vs s <=> assn_of_vs s'.
+  Proof.
+    remember (SE.cardinal s) as car_s eqn:Heqc.
+    revert s s' Heqc; induction car_s using lt_wf_ind; intros s s' Heqc Heqss'.
+    destruct car_s.
+    - assert (SE.Empty s).
+      { unfold SE.Empty; intros.
+        rewrite SE.cardinal_spec in Heqc.
+        destruct s as [[|? ?] ?]; simpl in *; try congruence.
+        cbv; inversion 1. }
+      forwards* : (eqset_empty).
+      forwards* Heq: (assn_empty s); rewrite Heq.
+      forwards* Heq': (assn_empty s'); rewrite Heq'; reflexivity.
+    - lets a Ha: (>>choose_card s); try omega.
+      assert (SE.In a s') by (applys* Heqss').
+      rewrites* (>>add_equiv' a s).
+      rewrites* (>>add_equiv' a s').
+      rewrites* (>>add_equiv (SE.remove a s)); [apply remove_nin|].
+      rewrites* (>>add_equiv (SE.remove a s')); [apply remove_nin|].
+      destruct (find a); [|reflexivity].
+      rewrites H; try reflexivity.
+      forwards*: (remove_card a s); omega.
+      apply (add_inverts a); eauto using remove_nin.
+      rewrite <-!choose_remove; eauto.
+  Qed.          
+
+  Instance eqset_proper stk : Proper (SE.Equal ==> equiv_sep stk) assn_of_vs.
+  Proof.
+    intros s1 s2 Heq; apply eqset_equiv; auto.
+  Qed.
+
+  Lemma union_add_l a s s' : SE.union (SE.add a s) s' == SE.add a (SE.union s s').
+  Proof.
+    simpl; unfold SE.Equal; intros.
+    repeat (try rewrite SE.union_spec; try rewrite SE.add_spec); intuition.
+  Qed.
+
+  Lemma union_add_r a s s' : SE.union s (SE.add a s') == SE.add a (SE.union s s').
+  Proof.
+    simpl; unfold SE.Equal; intros.
+    repeat (try rewrite SE.union_spec; try rewrite SE.add_spec); intuition.
+  Qed.
+  
+  Lemma union_assns s s' stk :
+    stk ||= 
+        assn_of_vs (SE.union s s') <=>
+        assn_of_vs s **
+        assn_of_vs (SE.diff s' s).
+  Proof.
+    remember (SE.cardinal s) as car_s eqn:Heqc.
+    revert s s' Heqc; induction car_s using lt_wf_ind; intros s s' Heqc.
+    destruct car_s.
+    - forwards*: cardinal0_empty'; substs.
+      rewrites (union_emp_l s').
+      rewrite assn_empty'.
+      rewrites (diff_emp_r s').
+      rewrite emp_unit_l; reflexivity.
+    - forwards* (a & Hin): (choose_card s); try omega.
+      forwards* Heq: (choose_remove s).
+      rewrite Heq at 1 2.
+      rewrite union_add_l, <-union_add_r.
+      rewrite (H car_s); try omega; try (rewrites* remove_card; omega).
+      assert (Heq' : SE.diff (SE.add a s') (SE.remove a s) ==
+                     SE.add a (SE.remove a (SE.diff s' s))).
+      { simpl; unfold SE.Equal; intros;
+        repeat (try rewrite SE.diff_spec;
+                try rewrite SE.add_spec;
+                try rewrite SE.remove_spec).
+        assert (Decidable.decidable (SE.In a0 s)).
+        { unfolds; destruct (SE.mem a0 s) eqn:Heq'.
+          rewrite SE.mem_spec in *; eauto.
+          right; intros Hc; rewrite <-SE.mem_spec in Hc; congruence. }
+        clear; intros; intuition.
+        destruct (eq_dec a0 a); eauto. }
+      rewrite Heq'.
+      repeat rewrite add_equiv; [|apply remove_nin..].
+      destruct (find a).
+      2: split; intros (? & ? & ? & ? & ? & ?); lazymatch goal with [H : False |- _] => destruct H end.
+      assert (Heq'' : SE.remove a (SE.diff s' s) == SE.diff s' s).
+      { simpl; unfold SE.Equal; intros;
+        repeat (try rewrite SE.diff_spec;
+                try rewrite SE.add_spec;
+                try rewrite SE.remove_spec).
+        intuition; subst; eauto. }
+      rewrite Heq''.
+      rewrite <-!sep_assoc; split; intros; repeat sep_cancel.
+  Qed.
+End VarsCondition.
+
 Section CorrectnessProof.
   Import Skel_lemma.
   (* the set of free variables *)
@@ -736,11 +1167,7 @@ Section CorrectnessProof.
   Variable BS : nat -> Vector.t assn ntrd * Vector.t assn ntrd.
   Arguments assn_of_svs _ _ _ _ _ : simpl never.
   Arguments assn_of_avs _ _ _ : simpl never.
-  Arguments flip / _ _ _ _ _ _.
-  Tactic Notation "simpl_avs" "in" hyp(HP) := unfold assn_of_svs, assn_of_avs, SE.fold in HP; simpl in HP.
-  Tactic Notation "simpl_avs" := unfold assn_of_svs, assn_of_avs, SE.fold; simpl.
-  Tactic Notation "simpl_avs" "in" "*" := unfold assn_of_svs, assn_of_avs, SE.fold in *; simpl in *.
-  
+
   Lemma compile_ok (se : SExp) (seval_env : Env varE (option SVal) _)
         (svar_env : Env varE (list var) _) (n m : nat)
         (sv : SVal) c es :
@@ -781,240 +1208,68 @@ Section CorrectnessProof.
       
       forwards*: IHse1.
 
-      Infix "==" := SE.Equal.
-
-      Lemma eqset_empty s s' : SE.Empty s -> s == s' -> SE.Empty s'.
-      Proof.
-        unfold not, SE.Empty, "=="; firstorder.
-      Qed.
-
-      Lemma assn_empty s seval_env svar_env stk : SE.Empty s -> stk ||= assn_of_svs seval_env svar_env s <=> emp.
-      Proof.
-        destruct s as [[| ? ?] ?]; rewrite <-SE.is_empty_spec; simpl; 
-          unfold SE.is_empty; simpl; try congruence.
-        simpl_avs; split; eauto.
-      Qed.
-
-      Lemma choose_remove s x : SE.In x s -> s == SE.add x (SE.remove x s).
-      Proof.
-        revert s x; clear; intros s x.
-        unfold "=="; intros.
-        rewrite SE.add_spec, SE.remove_spec.
-        lets [? | ?]: (VarE_eq.eq_dec a x); split; intros; substs; intuition.
-        substs; eauto.
-      Qed.
-
-      Lemma equal_in x s s' : SE.In x s -> s == s' -> SE.In x s'.
-      Proof.
-        unfold "==", SE.In; intros.
-        rewrite <-H0; auto.
-      Qed.
-
-      Lemma cardinal0_empty s : SE.cardinal s = 0 <-> SE.Empty s.
-      Proof.
-        unfold SE.Empty, SE.cardinal; intros; split; intros H.
-        - destruct s as [[|? ?] ?]; simpl in *; try congruence.
-          cbv; inversion 1.
-        - destruct s as [[| ? ? ] ?]; simpl; auto.
-          false; lets: (H e); apply H0; left; auto.
-      Qed.
-
-      Lemma cardinal_add x s : ~SE.In x s -> SE.cardinal (SE.add x s) = S (SE.cardinal s).
-      Proof.
-        destruct s as [s ?]; unfold SE.In, SE.add, SE.cardinal; simpl.
-        remember (SE.Raw.cardinal s) as car_s eqn:Heqc.
-        clear is_ok.
-        revert s Heqc; induction car_s using lt_wf_ind; intros s Heqc Hnin.
-        destruct car_s.
-        - unfold SE.cardinal in *; destruct s as [|? ?]; simpl in *; congruence.
-        - unfold SE.cardinal in *; destruct s as [|? ?]; simpl in *; try congruence.
-          destruct VarE_eq.eq_dec; unfold VarE_eq.eq in *; simpl in *; substs.
-          + false; unfold SE.Raw.In in Hnin; apply Hnin.
-            constructor; auto.
-          + forwards* :(>>H car_s s).
-            intros Hc; apply Hnin; right; auto.
-      Qed.  
-
-      Lemma remove_nin x s : ~SE.In x (SE.remove x s).
-      Proof.
-        rewrite SE.remove_spec; intros [? ?]; congruence.
-      Qed.
-
-      Lemma eqset_cardinal s s' : s == s' -> SE.cardinal s = SE.cardinal s'.
-      Proof.
-        destruct s as [s oks], s' as [s' oks'].
-        unfold "==", SE.In, SE.cardinal; simpl.
-        revert s' oks'; induction s; simpl in *; intros s' oks'.
-        - destruct s'; simpl; auto.
-          intros H; lets [? ?]: (H e); unfold SE.Raw.In in *; simpl in *.
-          false; forwards: H1; [left; auto|inversion H2].
-        - intros Heq.
-          inverts oks.
-          assert (SE.Raw.Ok s) by apply H2.
-          cutrewrite (SE.Raw.cardinal s' = S (SE.Raw.cardinal (SE.Raw.remove a s'))).
-          erewrite IHs; eauto using SE.Raw.remove_ok.
-          { intros b; rewrite SE.Raw.remove_spec; eauto.
-            split; intros.
-            + split.
-              rewrite <-Heq; right; auto.
-              intros Hc; substs; unfold SE.Raw.In in *; auto.
-            + destruct H0.
-              rewrite <-Heq in H0; inverts H0; try congruence.
-              unfold SE.Raw.In; auto. }
-          { assert (SE.Raw.In a s').
-            { rewrite <-Heq; left; auto. }
-            revert H0 oks'; clear.
-            induction s'; simpl.
-            - inversion 1.
-            - destruct VarE_eq.eq_dec as [Heq | Heq]; unfold VarE_eq.eq in Heq; substs; auto.
-              simpl.
-              intros; rewrite <-IHs'; eauto.
-              inversion H0; substs; eauto; congruence.
-              inversion oks'; substs; auto. }
-      Qed.
-
-      Lemma eqset_remove a s s' : s == s' -> SE.remove a s == SE.remove a s'.
-      Proof.
-        unfold "=="; intros; rewrite !SE.remove_spec.
-        firstorder.
-      Qed.
-
-      Lemma add_eq a s :
-        ~In a s ->
-        SE.Raw.add a s = s ++ a :: nil.
-      Proof.
-        induction s; simpl; eauto.
-        intros Hc.
-        destruct VarE_eq.eq_dec; simpl.
-        - false; apply Hc; left; auto.
-        - f_equal; rewrite IHs; auto.
-      Qed.
-
-      Lemma add_equiv seval_env svar_env a s stk :
-        ~SE.In a s ->
-        stk ||= assn_of_svs seval_env svar_env (SE.add a s) <=>
-            match seval_env a with
-            | Some v => !((vars2es (svar_env a)) ==t vs_of_sval v) ** assn_of_svs seval_env svar_env s
-            | None => FalseP 
-            end.
-      Proof.
-        unfold assn_of_svs, SE.add, SE.In; rewrite !SE.fold_spec.
-        destruct s as [s oks]; simpl.
-        intros; rewrite add_eq; [|intros Hc; eapply In_InA in Hc; eauto using SE.E.eq_equiv].
-        rewrite fold_left_app; simpl.
-        destruct (seval_env a); [|reflexivity].
-        reflexivity.
-      Qed.        
-
-      Lemma add_remove_equiv seval_env svar_env a s stk :
-        SE.In a s ->
-        stk ||= assn_of_svs seval_env svar_env (SE.add a (SE.remove a s)) <=>
-                assn_of_svs seval_env svar_env s.
-      Proof.
-      Admitted.
-
-      Lemma eqset_equiv seval_env svar_env s s' stk :
-        SE.Equal s s' ->
-        stk ||= assn_of_svs seval_env svar_env s <=> assn_of_svs seval_env svar_env s'.
-      Proof.
-        remember (SE.cardinal s) as car_s eqn:Heqc.
-        revert s s' Heqc; induction car_s using lt_wf_ind; intros s s' Heqc Heqss'.
-        destruct car_s.
-        - assert (SE.Empty s).
-          { unfold SE.Empty; intros.
-            rewrite SE.cardinal_spec in Heqc.
-            destruct s as [[|? ?] ?]; simpl in *; try congruence.
-            cbv; inversion 1. }
-          forwards* : (eqset_empty).
-          forwards* Heq: (assn_empty s); rewrite Heq.
-          forwards* Heq': (assn_empty s'); rewrite Heq'; reflexivity.
-        - destruct (SE.choose s) as [a |] eqn:Hchoose.
-          forwards*: SE.choose_spec1.
-          forwards* Heq: choose_remove.
-          assert (SE.cardinal s = S (SE.cardinal (SE.remove a s))).
-          { lets: (remove_nin a s).
-            rewrites (>>eqset_cardinal Heq).
-            rewrites cardinal_add; eauto using remove_nin. }
-          forwards*: (>>H (SE.cardinal (SE.remove a s)) (SE.remove a s) (SE.remove a s')); try omega;
-            eauto using eqset_remove.
-          assert (SE.In a s') by eauto using equal_in.
           
-          
-          
-          { apply SE.choose_spec2 in Hchoose.
-            rewrite <-cardinal0_empty in Hchoose; congruence. }
-      Qed.          
-        
 
-      Lemma union_emp_l s : SE.Equal (SE.union s SE.empty) s.
-      Proof.
-        unfold SE.Equal; intros a.
-        rewrite SE.union_spec.
-        lets: (SE.empty_spec); unfold SE.Empty in H.
-        split; [intros [|]|intros]; eauto.
-        intros; false; eapply H; eauto.
-      Qed.
+      (* Lemma uniq_subset A (eqt : eq_type A) (xs ys : list A) : *)
+      (*   incl xs ys -> incl (uniq xs) (uniq ys). *)
+      (* Proof. *)
+      (*   revert ys; functional induction (uniq xs); unfold incl; simpl; intros ys Hin z Hinz; *)
+      (*     destruct Hinz; substs. *)
+      (*   - forwards *: (Hin z). *)
+      (*     apply uniq_incl'; eauto. *)
+      (*   - apply IHl; eauto. *)
+      (*     unfold incl; intros; apply Hin. *)
+      (*     right. *)
+      (*     lets: remove_incl; unfold incl in *; eauto. *)
+      (* Qed. *)
 
-      Lemma uniq_subset A (eqt : eq_type A) (xs ys : list A) :
-        incl xs ys -> incl (uniq xs) (uniq ys).
-      Proof.
-        revert ys; functional induction (uniq xs); unfold incl; simpl; intros ys Hin z Hinz;
-          destruct Hinz; substs.
-        - forwards *: (Hin z).
-          apply uniq_incl'; eauto.
-        - apply IHl; eauto.
-          unfold incl; intros; apply Hin.
-          right.
-          lets: remove_incl; unfold incl in *; eauto.
-      Qed.
-
-      Lemma assn_of_svs_subset xs ys (seval_env : Env varE (option SVal) _) (svar_env : Env varE (list var) _) stk :
-        incl xs ys ->
-        exists zs,
-          stk ||= !(assn_of_svs seval_env svar_env ys) <=>
-                  !(assn_of_svs seval_env svar_env xs) ** !(assn_of_svs seval_env svar_env zs).
-      Proof.
-        revert xs; induction ys; simpl; unfold incl; intros xs Hin.
-        - assert (xs = nil); [|substs].
-          { destruct xs; eauto; simpl in *.
-            forwards* : (Hin v). }
-          exists (@nil varE); simpl.
-          split; intros; sep_split_in H; sep_split; eauto.
-        - simpl in Hin.
-          assert (incl (remove eq_dec a xs) ys).
-          { unfold incl; intros b Hin'.
-            destruct (eq_dec a b) as [|Hneq]; substs.
-            - apply remove_In in Hin' as [].
-            - forwards* : (Hin b).
-              Lemma remove_neq' a b xs :
-                a <> b -> In a (remove eq_dec b xs) -> In a xs.
-              Proof.
-                induction xs; simpl; eauto.
-                destruct eq_dec; eauto.
-                simpl; intros ? [? | ?]; eauto.
-              Qed.
-              eapply remove_neq'; eauto. }
-          forwards* [zs IH]: (>>IHys H).
+      (* Lemma assn_of_svs_subset xs ys (seval_env : Env varE (option SVal) _) (svar_env : Env varE (list var) _) stk : *)
+      (*   incl xs ys -> *)
+      (*   exists zs, *)
+      (*     stk ||= !(assn_of_svs seval_env svar_env ys) <=> *)
+      (*             !(assn_of_svs seval_env svar_env xs) ** !(assn_of_svs seval_env svar_env zs). *)
+      (* Proof. *)
+      (*   revert xs; induction ys; simpl; unfold incl; intros xs Hin. *)
+      (*   - assert (xs = nil); [|substs]. *)
+      (*     { destruct xs; eauto; simpl in *. *)
+      (*       forwards* : (Hin v). } *)
+      (*     exists (@nil varE); simpl. *)
+      (*     split; intros; sep_split_in H; sep_split; eauto. *)
+      (*   - simpl in Hin. *)
+      (*     assert (incl (remove eq_dec a xs) ys). *)
+      (*     { unfold incl; intros b Hin'. *)
+      (*       destruct (eq_dec a b) as [|Hneq]; substs. *)
+      (*       - apply remove_In in Hin' as []. *)
+      (*       - forwards* : (Hin b). *)
+      (*         Lemma remove_neq' a b xs : *)
+      (*           a <> b -> In a (remove eq_dec b xs) -> In a xs. *)
+      (*         Proof. *)
+      (*           induction xs; simpl; eauto. *)
+      (*           destruct eq_dec; eauto. *)
+      (*           simpl; intros ? [? | ?]; eauto. *)
+      (*         Qed. *)
+      (*         eapply remove_neq'; eauto. } *)
+      (*     forwards* [zs IH]: (>>IHys H). *)
 
               
 
-          Lemma assn_of_svs_equiv xs ys (seval_env : Env varE (option SVal) _) (svar_env : Env varE (list var) _) stk :
-            equiv_ls _ xs ys ->
-            stk ||= !(assn_of_svs seval_env svar_env xs) <=> !(assn_of_svs seval_env svar_env ys).
-          Proof.
-            revert ys; induction xs; simpl; simpl; intros ys Heq.
-            - assert (ys = nil); [|substs; simpl].
-              { unfold equiv_ls, incl in Heq; destruct Heq, ys; simpl in *; eauto.
-                forwards*: (H0 v). }
-              reflexivity.
-            - destruct ys as [|y ys].
-              { unfold equiv_ls, incl in Heq; destruct Heq; simpl in *.
-                forwards*: (H a). }
+      (*     Lemma assn_of_svs_equiv xs ys (seval_env : Env varE (option SVal) _) (svar_env : Env varE (list var) _) stk : *)
+      (*       equiv_ls _ xs ys -> *)
+      (*       stk ||= !(assn_of_svs seval_env svar_env xs) <=> !(assn_of_svs seval_env svar_env ys). *)
+      (*     Proof. *)
+      (*       revert ys; induction xs; simpl; simpl; intros ys Heq. *)
+      (*       - assert (ys = nil); [|substs; simpl]. *)
+      (*         { unfold equiv_ls, incl in Heq; destruct Heq, ys; simpl in *; eauto. *)
+      (*           forwards*: (H0 v). } *)
+      (*         reflexivity. *)
+      (*       - destruct ys as [|y ys]. *)
+      (*         { unfold equiv_ls, incl in Heq; destruct Heq; simpl in *. *)
+      (*           forwards*: (H a). } *)
               
 
-          exists zs; simpl.
-          destruct (seval_env a).
-          2: split; intros H'; sep_split_in H'; sep_split; try destruct HP; eauto.
-          rewrite !pure_star, !pure_pure.
-          rewrite IH.
-          split; intros; repeat sep_cancel.
+      (*     exists zs; simpl. *)
+      (*     destruct (seval_env a). *)
+      (*     2: split; intros H'; sep_split_in H'; sep_split; try destruct HP; eauto. *)
+      (*     rewrite !pure_star, !pure_pure. *)
+      (*     rewrite IH. *)
+      (*     split; intros; repeat sep_cancel. *)
